Redefined epsilon NFA's

src/NFA.lean
@@ -1,6 +1,7 @@
 import data.fintype.basic
 import data.set.lattice
 import DFA
+import fixpoint
 
 universes u v
 
@@ -110,3 +111,121 @@ lemma DFA_of_NFA_correct (M : NFA) (s : list M.alphabet) :
   M.accepts s ↔ M.DFA_of_NFA.accepts s := by refl
 
 end NFA
+
+structure ε_NFA := 
+(alphabet : Type u) 
+[alphabet_fintype : fintype alphabet]
+(state : Type v)
+[state_fintype : fintype state]
+(step : state → option alphabet → set state)
+(start : set state)
+(accept_states : set state)
+
+namespace ε_NFA
+
+instance fin₁ (M : ε_NFA) : fintype M.alphabet := M.alphabet_fintype
+instance fin₂ (M : ε_NFA) : fintype M.state := M.state_fintype
+
+open least_fixpoint
+
+inductive in_ε_closure (M : ε_NFA) : set M.state → M.state → Prop
+| base : ∀ Ss (S ∈ Ss), in_ε_closure Ss S
+| step : ∀ Ss S (h : in_ε_closure Ss S), in_ε_closure (Ss >>= (λ (T : M.state), M.step T option.none)) S
+
+inductive ε_closure (M : ε_NFA) : set M.state → M.state → Prop
+| base : ∀ Ss (S ∈ Ss), ε_closure Ss S
+| step : ∀ Ss S T, ε_closure Ss S → T ∈ M.step S option.none → ε_closure Ss T
+
+-- def ε_closure (M : ε_NFA) (Ss : set M.state) : set M.state :=
+-- set_of (least_fixpoint (λ Ts, Ts ∪ (Ts >>= (λ (T : M.state), M.step T option.none))) Ss)
+
+-- @[simp] lemma ε_closure_of_ε_closure (M : ε_NFA) :
+--   ∀ (Ss : set M.state), M.ε_closure (M.ε_closure Ss) = M.ε_closure Ss := 
+-- -- fixpoint_of_fixpoint _ begin simp end
+-- begin
+--   intro Ss,
+--   ext S,
+--   split,
+--   { intro h,
+--     type_check ε_closure.rec_on h,
+--     -- generalize_hyp ha : M.ε_closure Ss = a at h,
+--     -- apply ε_closure.base,
+--     induction h with _ _ _ Ss S' T hT h ih,
+--     { finish },
+--     {  } },
+--   { intro h,
+--     apply ε_closure.base,
+--     assumption }
+-- end
+
+def step_set (M : ε_NFA) : set M.state → M.alphabet → set M.state :=
+λ Ss a, M.ε_closure $ Ss >>= λ S, M.step S (option.some a)
+
+def eval (M : ε_NFA) : list M.alphabet → set M.state := list.foldl M.step_set (M.ε_closure M.start)
+
+def accepts (M : ε_NFA) (s : list M.alphabet) : Prop :=
+∃ S ∈ M.accept_states, S ∈ M.eval s
+
+def NFA_of_ε_NFA (M : ε_NFA) : NFA :=
+{ alphabet := M.alphabet,
+  state := M.state,
+  step := λ S a, M.ε_closure (M.step S (some a)),
+  start := M.ε_closure M.start,
+  accept_states := M.accept_states }
+
+lemma NFA_of_ε_NFA_step_set_match (M : ε_NFA) (Ss : set M.state) (a : M.alphabet) :
+  M.step_set Ss a = M.NFA_of_ε_NFA.step_set Ss a :=
+begin
+  rw [step_set, NFA.step_set],
+  simp, 
+  change M.ε_closure (⋃ (i : M.state) (H : i ∈ Ss), M.step i (some a)) = ⋃ (i : M.NFA_of_ε_NFA.state) (H : i ∈ Ss), M.ε_closure (M.step i (some a)),
+  ext b,
+  split,
+  { intro h,   
+    generalize_hyp hT : (⋃ (i : M.state) (H : i ∈ Ss), M.step i (some a)) = Ts at h,
+    induction h with _ _ h Us U T hU h ih,
+    { rw ←hT at h,
+      simp only [exists_prop, set.mem_Union] at h ⊢,
+      cases h with i hi,
+      use i,
+      use hi.1,
+      apply ε_closure.base,
+      tauto },
+    { simp only [exists_prop, set.mem_Union] at *,
+      specialize ih hT,
+      cases ih with i ih,
+      existsi i,
+      existsi ih.1,
+      apply ε_closure.step,
+      use ih.2,
+      assumption } },
+  { rintro ⟨ _, ⟨ ⟨ S, rfl ⟩, hb ⟩ ⟩,
+    simp only [exists_prop, set.mem_Union] at hb,
+    cases hb with hS h,
+    generalize_hyp hT : M.step S (some a) = T at h,
+    induction h,
+    { apply ε_closure.base,
+      finish },
+    { specialize h_ih hT,
+      apply ε_closure.step,
+      assumption' } }
+end
+
+lemma NFA_of_ε_NFA_eval_match (M : ε_NFA) (s : list M.alphabet) :
+  M.eval s = (NFA_of_ε_NFA M).eval s :=
+begin
+  change list.foldl M.step_set (M.ε_closure M.start) s = list.foldl M.NFA_of_ε_NFA.step_set (M.ε_closure M.start) s,
+  congr,
+  ext1,
+  ext1,
+  rw NFA_of_ε_NFA_step_set_match
+end
+
+lemma NFA_of_ε_NFA_correct (M : ε_NFA) (s : list M.alphabet) :
+  M.accepts s ↔ M.NFA_of_ε_NFA.accepts s :=
+begin
+  rw [accepts, NFA.accepts, NFA_of_ε_NFA_eval_match],
+  tauto
+end
+
+end ε_NFA
